Lyule/Theorems.lean
@@ -2,6 +2,8 @@ import Lyule.Semantics
 import Lyule.Syntax 
 import Lyule.Utils
 
+import Aesop 
+
 -- Lemma 2 of Amin and Rompf paper. 
 -- lemma: well-typed lookups are not stuck and preserves types 
 -- This proof is immediate because this property is ensured by 
@@ -12,9 +14,43 @@ lemma lookupVarLemma {ctx t}
   intros env p 
   exists (lookupVar p env)
 
+-- well typed lookup lemma for functions 
+
 lemma lookupFunLemma {fctx s} 
   : ∀ (fenv : Functions fctx)(p : Idx s fctx), ∃ f : Func fctx s, 
       lookupAll fenv p = f := by 
     intros fenv p
     exists (lookupAll fenv p) 
+
+-- Lemma 3 of Amin and Rompf paper 
+
+lemma evalLemma 
+  : ∀ (n : Fuel)(prog : Program)(p : Σ ctx, Env ctx),  
+      evalProg n prog = .Ok p → 
+      ∃ (ctx : Ctx)(env : Env ctx), p = Sigma.mk _ env := by
+      intros n 
+      induction n with 
+      | zero => 
+        intros _prog p 
+        simp [evalProg] 
+        aesop  
+      | succ n' _IH => 
+        intros _prog p _H 
+        exists p.1
+        exists p.2
+
+-- type soundness lemma 
+
+theorem soundness 
+  : ∀ n prog p, evalProg n prog = p → (∃ (ctx : Ctx)(env : Env ctx), p = .Ok (Sigma.mk ctx env)) ∨ 
+                                      p = .Timeout := by 
+      intros n prog p H 
+      rcases p with ⟨ ctx , env ⟩ | _ 
+      · 
+        left 
+        exists ctx 
+        exists env 
+      · 
+        right 
+        rfl  
 
